Prove invariance w.r.t. preprepare

src/program_proof/rsm/distx/res.v
@@ -223,7 +223,7 @@ Section res.
   Definition txnwrs_frag γ (ts : nat) (dq : dfrac) (owrs : option dbmap) : iProp Σ.
   Admitted.
 
-  Definition txnwrs_frag_excl γ (ts : nat) :=
+  Definition txnwrs_excl γ (ts : nat) :=
     txnwrs_frag γ ts (DfracOwn 1) None.
 
   Definition txnwrs_receipt γ (ts : nat) (wrs : dbmap) :=
@@ -234,23 +234,39 @@ Section res.
     Persistent (txnwrs_receipt γ ts wrs).
   Admitted.
 
-  Lemma txnwrs_allocate γ owrsm ts :
-    owrsm !! ts = None ->
-    txnwrs_auth γ owrsm ==∗
-    txnwrs_auth γ (<[ts := None]> owrsm) ∗ txnwrs_frag_excl γ ts.
+  Lemma txnwrs_allocate γ wrsm ts :
+    wrsm !! ts = None ->
+    txnwrs_auth γ wrsm ==∗
+    txnwrs_auth γ (<[ts := None]> wrsm) ∗ txnwrs_excl γ ts.
   Admitted.
 
-  Lemma txnwrs_set γ owrsm ts wrs :
-    txnwrs_auth γ owrsm -∗
-    txnwrs_frag_excl γ ts ==∗
-    txnwrs_auth γ (<[ts := Some wrs]> owrsm) ∗ txnwrs_receipt γ ts wrs.
+  Lemma txnwrs_set γ wrsm ts wrs :
+    txnwrs_excl γ ts -∗
+    txnwrs_auth γ wrsm ==∗
+    txnwrs_auth γ (<[ts := Some wrs]> wrsm) ∗ txnwrs_receipt γ ts wrs.
   Admitted.
 
-  Lemma txnwrs_lookup γ owrsm ts wrs :
-    txnwrs_auth γ owrsm -∗
+  Lemma txnwrs_frag_lookup γ wrsm ts dq owrs :
+    txnwrs_frag γ ts dq owrs -∗
+    txnwrs_auth γ wrsm -∗
+    ⌜wrsm !! ts = Some owrs⌝.
+  Admitted.
+
+  Lemma txnwrs_receipt_lookup γ wrsm ts wrs :
     txnwrs_receipt γ ts wrs -∗
-    ⌜owrsm !! ts = Some (Some wrs)⌝.
-  Admitted.
+    txnwrs_auth γ wrsm -∗
+    ⌜wrsm !! ts = Some (Some wrs)⌝.
+  Proof. iIntros "#Hwrs Hwrsm". by iApply txnwrs_frag_lookup. Qed.
+
+  Lemma txnwrs_excl_elem_of γ wrsm ts :
+    txnwrs_excl γ ts -∗
+    txnwrs_auth γ wrsm -∗
+    ⌜ts ∈ dom wrsm⌝.
+  Proof.
+    iIntros "Hwrs Hwrsm".
+    iDestruct (txnwrs_frag_lookup with "Hwrs Hwrsm") as %Hlookup.
+    by apply elem_of_dom_2 in Hlookup.
+  Qed.
 
   Lemma txnwrs_receipt_agree γ ts wrs1 wrs2 :
     txnwrs_receipt γ ts wrs1 -∗
