src/program_proof/rsm/distx/invariance/preprepare.v
@@ -1,0 +1,30 @@
+From Perennial.program_proof.rsm.distx Require Import prelude.
+
+Section inv.
+  Context `{!distx_ghostG Σ}.
+
+  Lemma txnsys_inv_preprepare γ Qr tid wrs :
+    valid_ts tid ->
+    valid_wrs wrs ->
+    Qr wrs ->
+    txnpost_receipt γ tid Qr -∗
+    txnwrs_excl γ tid -∗
+    txnsys_inv γ ==∗
+    txnsys_inv γ ∗
+    txnwrs_receipt γ tid wrs.
+  Proof.
+    iIntros (Hvts Hvwrs HQ) "#HQ Hexclwrs Htxn".
+    iNamed "Htxn".
+    iDestruct (txnwrs_excl_elem_of with "Hexclwrs Hwrsm") as %Hin.
+    iMod (txnwrs_set _ _ _ wrs with "Hexclwrs Hwrsm") as "[Hwrsm #Hwrs]".
+    iFrame "∗ # %".
+    rewrite wrsm_dbmap_insert_Some.
+    iModIntro.
+    iSplit.
+    { iApply big_sepM_insert_2; [iFrame "# %" | done]. }
+    iPureIntro.
+    split; first set_solver.
+    by apply map_Forall_insert_2.
+  Qed.
+
+End inv.
